src/ByteString.v
@@ -17,31 +17,32 @@ Definition appendS := "append".
 Definition ByteStringSpec := Def ADT {
   rep := list Word,
 
-  Def Constructor0 emptyS : rep := ret []%list,,
+  Def Constructor0 emptyS : rep := ret []%list,
 
-  Def Method1 consS (r : rep) (w : Word) : rep * unit :=
-    ret (cons w r, tt),
+  Def Method1 consS (r : rep) (w : Word) : rep :=
+    ret (cons w r),
+
   Def Method0 unconsS (r : rep) : rep * (option Word) :=
     ret (match r with
          | nil => (r, None)
          | cons x xs => (xs, Some x)
          end),
 
-  Def Method1 appendS (r1 : rep) (r2 : rep) : rep * unit :=
-    ret ((r1 ++ r2)%list, tt)
+  Def Binary Method0 appendS (r1 : rep) (r2 : rep) : rep :=
+    ret (r1 ++ r2)%list
 
 }%ADTParsing.
 
 Definition ByteString := Rep ByteStringSpec.
 
 Definition empty : Comp ByteString :=
-  Eval simpl in callCons ByteStringSpec emptyS.
+  Eval simpl in callMeth ByteStringSpec emptyS.
 
 Definition cons (w : Word) (bs : ByteString) : Comp ByteString :=
-  Eval simpl in (p <- callMeth ByteStringSpec consS bs w; ret (fst p)).
+  Eval simpl in (callMeth ByteStringSpec consS bs w).
 
 Definition uncons (bs : ByteString) : Comp (ByteString * option Word) :=
   Eval simpl in callMeth ByteStringSpec unconsS bs.
 
-Definition append (bs1 bs2 : ByteString) : Comp (ByteString * unit) :=
+Definition append (bs1 bs2 : ByteString) : Comp ByteString :=
   Eval simpl in callMeth ByteStringSpec appendS bs1 bs2.
